src/proof/well_formed.v
@@ -1,0 +1,43 @@
+Require Export New.proof.sync.
+From proof.k8s_io.api.apps Require Export v1_init.
+From proof.k8s_io.api.core Require Export v1_init.
+From proof.k8s_io.apimachinery.pkg.apis.meta Require Export v1_init.
+From proof Require Import prelude empty_ffi.
+From proof Require Export deepcopy.
+
+
+Section proof.
+Context `{hG: !heapGS Σ} {go_ctx: GoContext}.
+
+Definition object_meta_well_formed (m: v1.ObjectMeta.t) : iProp Σ :=
+  ⌜ m.(v1.ObjectMeta.UID') ≠ "_ORPHAN_POD"%go ⌝.
+
+Definition pod_well_formed (pod: v1.Pod.t) : iProp Σ :=
+  object_meta_well_formed pod.(v1.Pod.ObjectMeta').
+
+Axiom pod_well_formed_for_creation: v1.Pod.t → iProp Σ.
+
+Definition pod_nn_well_formed (pod: v1.Pod.t) (namespace name: go_string) : iProp Σ :=
+  ⌜ pod.(v1.Pod.ObjectMeta').(v1.ObjectMeta.Namespace') = namespace ⌝ ∗
+  ⌜ pod.(v1.Pod.ObjectMeta').(v1.ObjectMeta.Name') = name ⌝ ∗
+  pod_well_formed pod.
+
+Definition replicaset_well_formed (rs: v1.ReplicaSet.t) : iProp Σ :=
+  object_meta_well_formed rs.(v1.ReplicaSet.ObjectMeta') ∗
+  ∃ (v: w32), rs.(v1.ReplicaSet.Spec').(v1.ReplicaSetSpec.Replicas') ↦ v ∗ ⌜ 0 ≤ sint.Z v ⌝.
+
+Definition replicaset_nn_well_formed (rs: v1.ReplicaSet.t) (namespace name: go_string) : iProp Σ :=
+  ⌜ rs.(v1.ReplicaSet.ObjectMeta').(v1.ObjectMeta.Namespace') = namespace ⌝ ∗
+  ⌜ rs.(v1.ReplicaSet.ObjectMeta').(v1.ObjectMeta.Name') = name ⌝ ∗
+  replicaset_well_formed rs.
+
+Lemma well_formed_preserved_by_deepcopy_replicaset rs1 rs2 namespace name:
+  deepcopy_of_replicaset rs1 rs2 -∗
+    replicaset_nn_well_formed rs1 namespace name -∗
+      deepcopy_of_replicaset rs1 rs2 ∗
+      replicaset_nn_well_formed rs1 namespace name ∗
+      replicaset_nn_well_formed rs2 namespace name.
+Proof.
+Admitted.
+
+End proof.
